cava/arrow-examples/Mux2_1.v
@@ -15,7 +15,7 @@
 (****************************************************************************)
 
 From Arrow Require Import Category ClosureConversion.
-From Cava Require Import Arrow.ArrowExport.
+From Cava Require Import Arrow.ArrowExport Arrow.CavaArrow.
 
 Require Import Coq.Strings.String.
 From Coq Require Import Lists.List.
@@ -25,12 +25,13 @@ Local Open Scope string_scope.
 
 Section notation.
   Import KappaNotation.
+  Local Open Scope kind_scope.
 
-  Section var.
-    Variable var: Kind -> Kind -> Type.
+  (* Section var.
+    Variable var: Kind -> Kind -> Type. *)
 
     Definition mux2_1
-    : CavaExpr var << Bit, << Bit, Bit >>, Unit >> Bit :=
+    : forall cava: Cava, << Bit, << Bit, Bit >>, Unit >> ~> Bit :=
     <[ \ sel ab =>
       let '(a,b) = ab in
       let sel_a = and sel a in
@@ -39,14 +40,12 @@ Section notation.
       let sel_out = or sel_a sel_b in
       sel_out
     ]>.
-  End var.
+  (* End var. *)
 End notation.
 
 Open Scope kind_scope.
-Definition mux2_1_arrow {cava: Cava}: << Bit, << Bit, Bit >> >> ~[cava]~> Bit
-  := to_arrow @mux2_1.
 
-Lemma mux2_1_is_combinational: wf_combinational mux2_1_arrow.
+Lemma mux2_1_is_combinational: wf_combinational (mux2_1 _).
 Proof. combinational_obvious. Qed.
 
 Require Import Cava.Types.
@@ -59,7 +58,7 @@ Definition mux2_1_Interface :=
      [].
 
 Definition mux2_1_netlist :=
-  makeNetlist mux2_1_Interface (@mux2_1_arrow NetlistCava).
+  makeNetlist mux2_1_Interface (arrow_netlist mux2_1).
 
 Definition mux2_1_tb_inputs : list (bool * (bool * bool)) := 
  [(false, (false, true));
@@ -72,7 +71,7 @@ Definition mux2_1_tb_inputs : list (bool * (bool * bool)) :=
 (* Using `evaluate_to_terms` for a nicer extracted value *)
 Definition mux2_1_tb_expected_outputs : list bool :=
 
- map (fun i => evaluate mux2_1_arrow mux2_1_is_combinational i) mux2_1_tb_inputs.
+ map (fun i => evaluate mux2_1 mux2_1_is_combinational i) mux2_1_tb_inputs.
 
 Definition mux2_1_tb :=
   testBench "mux2_1_tb" mux2_1_Interface
